First draft of request-response functions

src/lib/communication/DY.Lib.Communication.API.fst
@@ -5,6 +5,7 @@ open DY.Core
 open DY.Lib.State.PKI
 open DY.Lib.State.PrivateKeys
 open DY.Lib.Event.Typed
+open DY.Lib.State.Typed
 
 #set-options "--fuel 0 --ifuel 0 --z3cliopt 'smt.qi.eager_threshold=100'"
 
@@ -47,8 +48,114 @@ type signature_input =
 instance parseable_serializeable_bytes_signature_input: parseable_serializeable bytes signature_input
   = mk_parseable_serializeable ps_signature_input
 
-(*** Events ***)
+// Response request pairs messages
+[@@with_bytes bytes]
+type request_message = {
+  id:bytes;
+  client:principal;
+  payload:bytes;
+  key:bytes
+}
 
+%splice [ps_request_message] (gen_parser (`request_message))
+%splice [ps_request_message_is_well_formed] (gen_is_well_formed_lemma (`request_message))
+
+instance parseable_serializeable_bytes_request_message: parseable_serializeable bytes request_message
+  = mk_parseable_serializeable ps_request_message
+
+[@@with_bytes bytes]
+type response_message = {
+  id:bytes;
+  payload:bytes
+}
+
+%splice [ps_response_message] (gen_parser (`response_message))
+%splice [ps_response_message_is_well_formed] (gen_is_well_formed_lemma (`response_message))
+
+instance parseable_serializeable_bytes_response_message: parseable_serializeable bytes response_message
+  = mk_parseable_serializeable ps_response_message
+
+[@@with_bytes bytes]
+type response_envelope = {
+  nonce:bytes;
+  ciphertext:bytes
+}
+
+%splice [ps_response_envelope] (gen_parser (`response_envelope))
+%splice [ps_response_envelope_is_well_formed] (gen_is_well_formed_lemma (`response_envelope))
+
+instance parseable_serializeable_bytes_response_envelope: parseable_serializeable bytes response_envelope
+  = mk_parseable_serializeable ps_response_envelope
+
+[@@with_bytes bytes]
+type authenticated_data = {
+  client:principal;
+  server:principal
+}
+
+%splice [ps_authenticated_data] (gen_parser (`authenticated_data))
+%splice [ps_authenticated_data_is_well_formed] (gen_is_well_formed_lemma (`authenticated_data))
+
+instance parseable_serializeable_bytes_authenticated_data: parseable_serializeable bytes authenticated_data
+  = mk_parseable_serializeable ps_authenticated_data
+
+
+(*** States ***)
+
+[@@with_bytes bytes]
+type client_send_request = {
+  id:bytes;
+  server:principal;
+  payload:bytes;
+  key:bytes
+}
+
+%splice [ps_client_send_request] (gen_parser (`client_send_request))
+%splice [ps_client_send_request_is_well_formed] (gen_is_well_formed_lemma (`client_send_request))
+
+[@@with_bytes bytes]
+type server_receive_request = {
+  id:bytes;
+  client:principal;
+  payload:bytes;
+  key:bytes
+}
+
+%splice [ps_server_receive_request] (gen_parser (`server_receive_request))
+%splice [ps_server_receive_request_is_well_formed] (gen_is_well_formed_lemma (`server_receive_request))
+
+[@@with_bytes bytes]
+type client_receive_response = {
+  id:bytes;
+  server:principal;
+  payload:bytes;
+  key:bytes
+}
+
+%splice [ps_client_receive_response] (gen_parser (`client_receive_response))
+%splice [ps_client_receive_response_is_well_formed] (gen_is_well_formed_lemma (`client_receive_response))
+
+[@@with_bytes bytes]
+type communication_states =
+  | ClientSendRequest: client_send_request -> communication_states
+  | ServerReceiveRequest: server_receive_request -> communication_states
+  | ClientReceiveResponse: client_receive_response -> communication_states
+
+#push-options "--ifuel 1"
+%splice [ps_communication_states] (gen_parser (`communication_states))
+%splice [ps_communication_states_is_well_formed] (gen_is_well_formed_lemma (`communication_states))
+#pop-options
+
+instance parseable_serializeable_bytes_communication_states: parseable_serializeable bytes communication_states
+  = mk_parseable_serializeable ps_communication_states
+
+instance local_state_communication_layer_session: local_state communication_states = {
+  tag = "DY.Lib.Communication.State";
+  format = parseable_serializeable_bytes_communication_states;
+}
+
+
+(*** Events ***)
 
 [@@with_bytes bytes]
 type communication_event =
@@ -58,6 +165,10 @@ type communication_event =
   | CommAuthReceiveMsg: sender:principal -> receiver:principal -> payload:bytes -> communication_event
   | CommConfAuthSendMsg: sender:principal -> receiver:principal -> payload:bytes -> communication_event
   | CommConfAuthReceiveMsg: sender:principal -> receiver:principal -> payload:bytes -> communication_event
+  | CommClientSendRequest: client:principal -> server:principal -> id:bytes -> payload:bytes -> communication_event
+  | CommServerReceiveRequest: server:principal -> id:bytes -> payload:bytes -> communication_event
+  | CommServerSendResponse: server:principal -> id:bytes -> payload:bytes -> communication_event
+  | CommClientReceiveResponse: client:principal -> server:principal -> id:bytes -> payload:bytes -> key:bytes -> communication_event
 
 #push-options "--ifuel 1 --fuel 0"
 %splice [ps_communication_event] (gen_parser (`communication_event))
@@ -69,10 +180,14 @@ instance event_communication_event: event communication_event = {
   format = mk_parseable_serializeable ps_communication_event;
 }
 
+
 (*** Layer Setup ***)
 
 val comm_layer_pkenc_tag: string
 let comm_layer_pkenc_tag = "DY.Lib.Communication.PkEnc.PublicKey"
+
+val comm_layer_aead_tag: string
+let comm_layer_aead_tag = "DY.Lib.Communication.Aead.Key"
 
 val comm_layer_sign_tag: string
 let comm_layer_sign_tag = "DY.Lib.Communication.Sign.PublicKey"
@@ -81,6 +196,9 @@ type communication_keys_sess_ids = {
   pki: state_id;
   private_keys: state_id;
 }
+
+val comm_label: principal -> principal -> label
+let comm_label sender receiver = join (principal_label sender) (principal_label receiver)
 
 
 (*** Communication Layer ***)
@@ -233,6 +351,89 @@ let receive_confidential_authenticated comm_keys_ids receiver msg_id =
   let*? cm:communication_message = return (verify_and_decrypt_message receiver msg_encrypted_signed_bytes sk_receiver vk_sender) in  
   trigger_event receiver (CommConfAuthReceiveMsg sender receiver cm.payload);*
   return (Some cm)
+
+(**** Request Response Pairs ****)
+
+val compute_request_message: principal -> bytes -> bytes -> bytes -> bytes
+let compute_request_message client id payload key =
+  let req:request_message = {client; id; payload; key} in
+  serialize request_message req
+
+val send_request:
+  communication_keys_sess_ids ->
+  principal -> principal -> bytes ->
+  traceful (option (state_id & timestamp))
+let send_request comm_keys_ids client server payload =
+  let* key = mk_rand (AeadKey comm_layer_aead_tag empty) (comm_label client server) 32 in
+  let* id = mk_rand NoUsage (join (principal_label client) (principal_label server)) 32 in
+  
+  let* sid = new_session_id client in
+  set_state client sid (ClientSendRequest {id; server; payload; key} <: communication_states);*
+  trigger_event client (CommClientSendRequest client server id payload);*
+  
+  let* req_payload = return (compute_request_message client id payload key) in
+  let*? msg_id = send_confidential comm_keys_ids client server req_payload in
+  return (Some (sid, msg_id))
+
+val decode_request_message: bytes -> option request_message
+let decode_request_message msg_bytes =
+  parse request_message msg_bytes
+
+val receive_request:
+  communication_keys_sess_ids ->
+  principal -> timestamp ->
+  traceful (option (state_id & bytes))
+let receive_request comm_keys_ids server msg_id =
+  let*? req_msg_bytes = receive_confidential comm_keys_ids server msg_id in
+  let*? req_msg:request_message = return (decode_request_message req_msg_bytes) in
+  let* sid = new_session_id server in
+  set_state server sid (ServerReceiveRequest {id=req_msg.id; client=req_msg.client; payload=req_msg.payload; key=req_msg.key} <: communication_states);*
+  trigger_event server (CommServerReceiveRequest server req_msg.id req_msg.payload);*
+  return (Some (sid, req_msg.payload))
+
+val compute_response_message: principal -> principal -> bytes -> bytes -> bytes -> bytes -> bytes
+let compute_response_message client server key nonce id payload =
+  let resp:response_message = {id; payload} in
+  let resp_bytes = serialize response_message resp in
+  let ad:authenticated_data = {client; server} in
+  let ad_bytes = serialize authenticated_data ad in
+  let ciphertext = aead_enc key nonce resp_bytes ad_bytes in
+  serialize response_envelope {nonce; ciphertext}
+
+val send_response:
+  communication_keys_sess_ids ->
+  principal -> state_id -> bytes -> traceful (option timestamp)
+let send_response comm_keys_ids server sid payload =
+  let*? state = get_state server sid in
+  guard_tr (ServerReceiveRequest? state);*?
+  let ServerReceiveRequest srr = state in
+  trigger_event server (CommServerSendResponse server srr.id payload);*
+  let* nonce = mk_rand NoUsage public 32 in
+  let resp_msg = compute_response_message srr.client server srr.key nonce srr.id payload in
+  let* msg_id = send_msg resp_msg in
+  return (Some msg_id)
+
+val decode_response: principal -> principal -> bytes -> bytes -> option response_message
+let decode_response client server key msg_bytes =
+  let? resp_env:response_envelope = parse response_envelope msg_bytes in
+  let ad:authenticated_data = {client; server} in
+  let ad_bytes = serialize authenticated_data ad in
+  let? resp_bytes = aead_dec key resp_env.nonce resp_env.ciphertext ad_bytes in
+  parse response_message resp_bytes
+
+val receive_response:
+  communication_keys_sess_ids ->
+  principal -> state_id -> timestamp ->
+  traceful (option response_message)
+let receive_response comm_keys_ids client sid msg_id =
+  let*? state = get_state client sid in
+  guard_tr (ClientSendRequest? state);*?
+  let ClientSendRequest csr = state in
+  let*? resp_msg_bytes = recv_msg msg_id in
+  let*? resp_msg:response_message = return (decode_response client csr.server csr.key resp_msg_bytes) in
+  set_state client sid (ClientReceiveResponse {id=csr.id; server=csr.server; payload=resp_msg.payload; key=csr.key} <: communication_states);*
+  trigger_event client (CommClientReceiveResponse client csr.server csr.id resp_msg.payload csr.key);*
+  return (Some resp_msg)
 
 
 (**** Layer Initialization ****)
